end of day 12/07/19

inference-tool/src/main/scala/inference/Config.scala
@@ -42,7 +42,7 @@ object Config {
         case "naive"           => (SelectionStrategies.naive_score _).curried
         case "rank"            => (SelectionStrategies.naive_score_outputs _).curried
         case "comprehensive"   => (SelectionStrategies.naive_score_comprehensive _).curried
-        case "comprehensiveEQ" => (SelectionStrategies.naive_score_comprehensive_eq_high _).curried
+        case "comprehensiveeq" => (SelectionStrategies.naive_score_comprehensive_eq_high _).curried
         case s =>
           throw new IllegalArgumentException(s"'${s}' is not a valid strategy ${Nondeterminisms.values}")
       }
